# asdf

$\AA$

asda

\begin{gather*}
	y_1 = x + 1 \\
	y_2 = x^2 - 1 \\
	x + 1 = x^2 - 1 \\
	x^2 - x - 2 = 0 \\
	(x - 2)(x + 1) = 0 \\
	x = -1, 2
\end{gather*}

```python
def main():
	print("hello")

main()
```

test


```c
int main() {
	printf("Hello world\n");
	return 0;
}
```

```c++
int main() {
	std::vector<float> t = {1, 2, 3, 4};
	return 0;
}
```

```go
func main() {
	go testFunc()
	x := 1
	fmt.Println(x)
}
```



![Fig. Random plot of stopping power](./Figure_4.svg)

![Fig. Random plot of stopping power](./Figure_4.svg)

asd

oasd

asd

asd

asd

asd
